whatever, stash

Rope.dfy
@@ -4,23 +4,41 @@ module BinaryTree {
   import opened Utils
   trait Node
   {
+    var left: Node?;
+    var right: Node?;
     var height: nat;
 
     function length(): nat
-      reads this
-      decreases this.height
+      reads this, this.right
+      decreases height
   }
 
   class NTNode extends Node
   {
+    ghost var Repr: set<object>
+
+    predicate Valid()
+      reads this, Repr
+      ensures Valid() ==> this in Repr
+    {
+      this in Repr &&
+      (this.left != null ==> this.left in Repr)
+    }
     var leftLen: nat;
-    var left: Node?;
-    var right: Node?;
+
+    predicate valid()
+      reads this, this.left, this.right
+    {
+      (this.left != null ==> this.leftLen == this.left.length()) &&
+      (this.left != null ==> this.height > this.left.height) &&
+      (this.right != null ==> this.height > this.right.height)
+    }
 
     constructor (left: Node, right: Node)
       ensures this.leftLen == left.length()
       ensures this.height > left.height
       ensures this.height > right.height
+      ensures this.height == max(left.height, right.height) + 1
     {
       this.left := left;
       this.right := right;
@@ -29,7 +47,8 @@ module BinaryTree {
     }
 
     function length(): nat
-      reads this
+      reads this, this.right
+      decreases height
     {
       this.leftLen + (if this.right == null then 0 else this.right.length())
     }
@@ -47,6 +66,7 @@ module BinaryTree {
 
     function length(): nat
       reads this
+      decreases height
     { |this.str| }
   }
 }
